atomics/lock.v
@@ -10,12 +10,12 @@ Module Info.
   Definition build_number := "".
   Definition build_tag := "".
   Definition build_branch := "".
-  Definition arch := "x86".
-  Definition model := "64".
-  Definition abi := "macos".
+  Definition arch := "aarch64".
+  Definition model := "default".
+  Definition abi := "apple".
   Definition bitsize := 64.
   Definition big_endian := false.
-  Definition source_file := "lock.c".
+  Definition source_file := "atomics/lock.c".
   Definition normalized := true.
 End Info.
 
@@ -25,6 +25,9 @@ Definition ___builtin_bswap : ident := $"__builtin_bswap".
 Definition ___builtin_bswap16 : ident := $"__builtin_bswap16".
 Definition ___builtin_bswap32 : ident := $"__builtin_bswap32".
 Definition ___builtin_bswap64 : ident := $"__builtin_bswap64".
+Definition ___builtin_cls : ident := $"__builtin_cls".
+Definition ___builtin_clsl : ident := $"__builtin_clsl".
+Definition ___builtin_clsll : ident := $"__builtin_clsll".
 Definition ___builtin_clz : ident := $"__builtin_clz".
 Definition ___builtin_clzl : ident := $"__builtin_clzl".
 Definition ___builtin_clzll : ident := $"__builtin_clzll".
@@ -35,6 +38,7 @@ Definition ___builtin_debug : ident := $"__builtin_debug".
 Definition ___builtin_expect : ident := $"__builtin_expect".
 Definition ___builtin_fabs : ident := $"__builtin_fabs".
 Definition ___builtin_fabsf : ident := $"__builtin_fabsf".
+Definition ___builtin_fence : ident := $"__builtin_fence".
 Definition ___builtin_fmadd : ident := $"__builtin_fmadd".
 Definition ___builtin_fmax : ident := $"__builtin_fmax".
 Definition ___builtin_fmin : ident := $"__builtin_fmin".
@@ -44,8 +48,6 @@ Definition ___builtin_fnmsub : ident := $"__builtin_fnmsub".
 Definition ___builtin_fsqrt : ident := $"__builtin_fsqrt".
 Definition ___builtin_membar : ident := $"__builtin_membar".
 Definition ___builtin_memcpy_aligned : ident := $"__builtin_memcpy_aligned".
-Definition ___builtin_read16_reversed : ident := $"__builtin_read16_reversed".
-Definition ___builtin_read32_reversed : ident := $"__builtin_read32_reversed".
 Definition ___builtin_sel : ident := $"__builtin_sel".
 Definition ___builtin_sqrt : ident := $"__builtin_sqrt".
 Definition ___builtin_unreachable : ident := $"__builtin_unreachable".
@@ -53,8 +55,6 @@ Definition ___builtin_va_arg : ident := $"__builtin_va_arg".
 Definition ___builtin_va_copy : ident := $"__builtin_va_copy".
 Definition ___builtin_va_end : ident := $"__builtin_va_end".
 Definition ___builtin_va_start : ident := $"__builtin_va_start".
-Definition ___builtin_write16_reversed : ident := $"__builtin_write16_reversed".
-Definition ___builtin_write32_reversed : ident := $"__builtin_write32_reversed".
 Definition ___compcert_i64_dtos : ident := $"__compcert_i64_dtos".
 Definition ___compcert_i64_dtou : ident := $"__compcert_i64_dtou".
 Definition ___compcert_i64_sar : ident := $"__compcert_i64_sar".
@@ -100,7 +100,7 @@ Definition f_makelock := {|
   (Scall (Some _t'1)
     (Evar _make_atomic (Tfunction (Tcons tint Tnil)
                          (tptr (Tstruct _atom_int noattr)) cc_default))
-    ((Econst_int (Int.repr 0) tint) :: nil))
+    ((Econst_int (Int.repr 1) tint) :: nil))
   (Sreturn (Some (Etempvar _t'1 (tptr (Tstruct _atom_int noattr))))))
 |}.
 
@@ -363,16 +363,22 @@ Definition global_definitions : list (ident * globdef fundef type) :=
                    (mksignature (AST.Tlong :: AST.Tlong :: nil) AST.Tlong
                      cc_default)) (Tcons tlong (Tcons tlong Tnil)) tlong
      cc_default)) ::
- (___builtin_fmax,
-   Gfun(External (EF_builtin "__builtin_fmax"
-                   (mksignature (AST.Tfloat :: AST.Tfloat :: nil) AST.Tfloat
-                     cc_default)) (Tcons tdouble (Tcons tdouble Tnil))
-     tdouble cc_default)) ::
- (___builtin_fmin,
-   Gfun(External (EF_builtin "__builtin_fmin"
-                   (mksignature (AST.Tfloat :: AST.Tfloat :: nil) AST.Tfloat
-                     cc_default)) (Tcons tdouble (Tcons tdouble Tnil))
-     tdouble cc_default)) ::
+ (___builtin_fence,
+   Gfun(External (EF_builtin "__builtin_fence"
+                   (mksignature nil AST.Tvoid cc_default)) Tnil tvoid
+     cc_default)) ::
+ (___builtin_cls,
+   Gfun(External (EF_builtin "__builtin_cls"
+                   (mksignature (AST.Tint :: nil) AST.Tint cc_default))
+     (Tcons tint Tnil) tint cc_default)) ::
+ (___builtin_clsl,
+   Gfun(External (EF_builtin "__builtin_clsl"
+                   (mksignature (AST.Tlong :: nil) AST.Tint cc_default))
+     (Tcons tlong Tnil) tint cc_default)) ::
+ (___builtin_clsll,
+   Gfun(External (EF_builtin "__builtin_clsll"
+                   (mksignature (AST.Tlong :: nil) AST.Tint cc_default))
+     (Tcons tlong Tnil) tint cc_default)) ::
  (___builtin_fmadd,
    Gfun(External (EF_builtin "__builtin_fmadd"
                    (mksignature
@@ -401,25 +407,16 @@ Definition global_definitions : list (ident * globdef fundef type) :=
                      AST.Tfloat cc_default))
      (Tcons tdouble (Tcons tdouble (Tcons tdouble Tnil))) tdouble
      cc_default)) ::
- (___builtin_read16_reversed,
-   Gfun(External (EF_builtin "__builtin_read16_reversed"
-                   (mksignature (AST.Tlong :: nil) AST.Tint16unsigned
-                     cc_default)) (Tcons (tptr tushort) Tnil) tushort
-     cc_default)) ::
- (___builtin_read32_reversed,
-   Gfun(External (EF_builtin "__builtin_read32_reversed"
-                   (mksignature (AST.Tlong :: nil) AST.Tint cc_default))
-     (Tcons (tptr tuint) Tnil) tuint cc_default)) ::
- (___builtin_write16_reversed,
-   Gfun(External (EF_builtin "__builtin_write16_reversed"
-                   (mksignature (AST.Tlong :: AST.Tint :: nil) AST.Tvoid
-                     cc_default)) (Tcons (tptr tushort) (Tcons tushort Tnil))
-     tvoid cc_default)) ::
- (___builtin_write32_reversed,
-   Gfun(External (EF_builtin "__builtin_write32_reversed"
-                   (mksignature (AST.Tlong :: AST.Tint :: nil) AST.Tvoid
-                     cc_default)) (Tcons (tptr tuint) (Tcons tuint Tnil))
-     tvoid cc_default)) ::
+ (___builtin_fmax,
+   Gfun(External (EF_builtin "__builtin_fmax"
+                   (mksignature (AST.Tfloat :: AST.Tfloat :: nil) AST.Tfloat
+                     cc_default)) (Tcons tdouble (Tcons tdouble Tnil))
+     tdouble cc_default)) ::
+ (___builtin_fmin,
+   Gfun(External (EF_builtin "__builtin_fmin"
+                   (mksignature (AST.Tfloat :: AST.Tfloat :: nil) AST.Tfloat
+                     cc_default)) (Tcons tdouble (Tcons tdouble Tnil))
+     tdouble cc_default)) ::
  (___builtin_debug,
    Gfun(External (EF_external "__builtin_debug"
                    (mksignature (AST.Tint :: nil) AST.Tvoid
@@ -454,10 +451,9 @@ Definition global_definitions : list (ident * globdef fundef type) :=
 Definition public_idents : list ident :=
 (_release :: _acquire :: _freelock :: _makelock :: _free_atomic ::
  _atom_CAS :: _atom_store :: _make_atomic :: ___builtin_debug ::
- ___builtin_write32_reversed :: ___builtin_write16_reversed ::
- ___builtin_read32_reversed :: ___builtin_read16_reversed ::
- ___builtin_fnmsub :: ___builtin_fnmadd :: ___builtin_fmsub ::
- ___builtin_fmadd :: ___builtin_fmin :: ___builtin_fmax ::
+ ___builtin_fmin :: ___builtin_fmax :: ___builtin_fnmsub ::
+ ___builtin_fnmadd :: ___builtin_fmsub :: ___builtin_fmadd ::
+ ___builtin_clsll :: ___builtin_clsl :: ___builtin_cls :: ___builtin_fence ::
  ___builtin_expect :: ___builtin_unreachable :: ___builtin_va_end ::
  ___builtin_va_copy :: ___builtin_va_arg :: ___builtin_va_start ::
  ___builtin_membar :: ___builtin_annot_intval :: ___builtin_annot ::
